<chapter xml:id="ch-4">
    <title>Higher order differential equations</title>
    <section xml:id="ch4-1">
        <title>Linear equations</title>
        <subsection>
        <title>General linear equations</title>
        <p>Everything we did in <xref ref="ch3" />for second order linear equations can be extended to higher order systems. Suppose we have the <m>n</m>th order linear equation 
        <me>
        a_{n}(t)y^{(n)}+a_{n-1}(t)y^{(n-1)}+\cdots+a_{1}(t)y^{\prime}+a_{0}(t)y=g(t).
        </me>
        We assume that <m>a_{n}(t),\dots,a_{0}(t)</m> are continuous functions
        on an interval <m>I</m>, and that <m>a_{n}(t)\neq0</m> inside the interval:
        so that we can write it in standand form as 
        <me>
        y^{(n)}+p_{n-1}(t)y^{(n-1)}+\cdots+p_{1}(t)y^{\prime}+p_{0}(t)y=g(t).\,\,\,\,\,(\star)
        </me>
        with initial conditions
        <me>
        y(t_{0})=y_{0},\,\,y^{\prime}(t_{0})=y_{0}^{\prime},\,\,\cdots,y^{(n-1)}(t_{0})=y_{0}^{(n-1)}.\,\,\,\,\,(\star)
        </me>.</p>

        <theorem><title>Existence/uniqueness</title> 
            <p> Let a linear differential equation be given in form <m>(\star)</m>.
            If <m>p_{n-1}(t),\dots,p_{0}(t)</m>
            are continuous functions on an open interval <m>I</m> (containing <m>t_{0}</m>),
            then there exists a unique solution <m>y=\phi(t)</m> throughout all of
            <m>I</m> to the IVP in <m>(\star)</m>.</p>
        </theorem> 

        <example>
            <p>Consider the ODE
            <me>
            (t-2)y^{(4)}+\sin ty^{\prime\prime\prime}+\ln ty=\sqrt{t+5}.
            </me>
            Find the intervals where you are guaranteed a unique solution to this
            ODE by the Uniqueness and Existence Theorem.</p>


            <p> Rewriting, we have 
            <me>
            y^{(4)}+\frac{\sin t}{(t-2)}y^{\prime\prime\prime}+\frac{\ln t}{(t-2)}y=\frac{\sqrt{t+5}}{(t-2)}
            </me>
            and 
            <ul>
                <li><m>\frac{\sin t}{(t-2)}</m> is comtinuous when <m>t\neq2</m></li>
                <li> <m>\frac{\ln t}{(t-2)}</m> is continuous when <m>t>0</m> and <m>t\neq2</m>, and </li>
                <li><m>\frac{\sqrt{t+5}}{(t-2)}</m> is continuous when <m>t\geq-5</m> and <m>t\neq2</m>. </li>
            </ul>
            Making a number line we see that all three functions are continuous
            when either on the interval <m>(0,2)</m> or <m>(2,\infty)</m>.</p>
        </example>
    </subsection>
    <subsection>
        <title>Constant coefficients</title>   
        <p>Now consider the homogeneous <m>n</m>th order linear equation with constant coefficients.
        <me>
        a_{n}y^{(n)}+a_{n-1}y^{(n-1)}+\cdots+a_{1}y^{\prime}+a_{0}y=0.
        </me> As we did in the <m>2</m>nd order case, the first thing we do is guess
        that the solution will look like <m>y=e^{rt}</m> and 
        <md>
        <mrow>y \amp =e^{rt}</mrow>
        <mrow>y^{\prime} \amp =re^{rt},</mrow>
        <mrow>\amp \vdots</mrow>
        <mrow>y^{(n)} \amp =r^{n}e^{rt}.</mrow>
        </md>
        Plugging into the LHS and setting equal to zero we have 
        <md>
        <mrow>LHS \amp =a_{n}\left(r^{n}e^{rt}\right)+\cdots+a_{1}\left(re^{rt}\right)+a_{0}\left(e^{rt}\right)</mrow>
         <mrow>\amp =e^{rt}\left(a_{n}r^{n}+\cdots+a_{0}\right)</mrow>
         <mrow>\amp =RHS=0</mrow>
        </md>
        hence 
        <me>
        e^{rt}\left(a_{n}r^{n}+\cdots+a_{0}\right)=0.
        </me>
        But since <m>e^{rt}\neq0</m> then 
        <me>
        a_{n}r^{n}+\cdots+a_{1}r+a_{0}=0.
        </me></p>

        <p>As before the <term>characteristic equation</term> is given by:
        <me>
        \begin{array}{c}
        \underbrace{a_{n}r^{n}+\cdots+a_{0}}\\
        Z(r)
        \end{array}=0,
        </me>
        where we call <m>Z(r)</m> the characteristic polynomial. How do we solve <m>n-</m>degree polynomials? By factoring! The fundamental theorem of algebra guarantees that an <m>n</m>th degree polynomial factors into <m>n</m> linear terms (assuming that we allow complex roots).
        <me>
        Z(t)=a_{n}\left(r-r_{1}\right)\left(r-r_{2}\right)\cdots\left(r-r_{n}\right).
        </me>
        <alert>HOWEVER</alert>, there is no general approach to factoring polynomials of degree greater than 4. Numerical techniques are necessary in these cases.</p>

        <p>Solutions to the ODE are built
        exactly like in the 2nd degree case. If there are any repeat solutions, then keep multiplying by <m>t</m> until
        you don't have any more repeat solutions.</p>
        <example> 
            <p>Find general solution and the particular
            solution to the IVP
            <me>
            y^{\prime\prime\prime}-2y^{\prime\prime}-y^{\prime}+2y=0.\,\,\,\,y(0)=0,y^{\prime}(0)=1,y^{\prime}(0)=2.
            </me>
            (Hint: Suppose you know <m>r^{3}-2r^{2}-r+2=\left(r-2\right)\left(r+1\right)\left(r-1\right)</m>)</p>

            <p> The characteristic equation is <m>2r^{3}-4r^{2}-2r+4=0</m>
            and by the hint we have
            <me>
            \left(r-2\right)\left(r+1\right)\left(r-1\right)=0,
            </me>
            hence the general solution is <m>y(t)=c_{1}e^{2t}+c_{2}e^{-t}+c_{3}e^{t}</m>.
            To find the particular solution to the IVP we start by:
            <md>
            <mrow>y(t) \amp =c_{1}e^{2t}+c_{2}e^{-t}+c_{3}e^{t}</mrow>
            <mrow>y^{\prime}(t) \amp =2c_{1}e^{2t}-c_{2}e^{-t}+c_{3}e^{t}</mrow>
            <mrow>y^{\prime\prime}(t) \amp =4c_{1}e^{2t}+c_{2}e^{-t}+c_{2}e^{t}.</mrow>
            </md>
            Then we have to solve the following system of equations:
            <md>
            <mrow>0 \amp =c_{1}+c_{2}+c_{3}</mrow>
            <mrow>1 \amp =2c_{1}-c_{2}+c_{3}</mrow>
            <mrow>2 \amp =4c_{1}+c_{2}+c_{3}</mrow>
            </md>
            and get <m>c_{1}=\frac{2}{3}</m>, <m>c_{2}=-\frac{1}{6}</m> and <m>c_{3}=-\frac{1}{2}</m>,
            hence 
            <me>
            y(t)=\frac{2}{3}e^{2t}-\frac{1}{6}e^{-t}-\frac{1}{2}e^{t}.
            </me></p>
        </example>

        <example> 
            <p>Find general solution of 
            <me>
            y^{(4)}+8y^{\prime\prime\prime}+16y^{\prime\prime}=0.
            </me>
            (Hint: <m>r^{4}+8r^{3}+16r^{2}=r^{2}\left(r+4\right)^{2}</m>)</p>
            
            <p>The characteristic polynomial is 
            <md>
            <mrow>r^{4}+8r^{3}+16r^{2} \amp =0</mrow>
            </md>
            which by the hint we know factors as
            <me>
            r^{2}\left(r+4\right)^{2}=0.
            </me>
            Note that since this a 4th degree polynomial we need to have 4 roots:
            <m>0,0,-4,-4</m>. So we use the same method we do when we have repeats
            and get 
            <md>
            <mrow>y(t) \amp =c_{1}e^{0t}+c_{2}te^{0t}+c_{3}e^{-4t}+c_{4}te^{-4t}</mrow>
             <mrow>\amp =c_{1}+c_{2}t+c_{3}e^{-4t}+c_{4}te^{-4t}.</mrow>
            </md></p>
        </example>

        <example>
            <p>Solve
            <me>
            y^{(4)}+y^{\prime\prime\prime}-5y^{\prime\prime}+y^{\prime}-6y=0.
            </me>
            (Hint: Suppose <m>\left(r-2\right)\left(r+3\right)\left(r^{2}+1\right)</m>)</p>

            <p>The characteristic equation is given
            by 
            <me>
            r^{4}+r^{3}-5r^{2}+r-6=0
            </me>
            and by the hint
            <me>
            Z(r)=\left(r-2\right)\left(r+3\right)\left(r^{2}+1\right)=0
            </me>
            which gives 
            <me>
            r=2,-3,\pm i
            </me>
            hence 
            <me>
            y(t)=c_{1}e^{2t}+c_{2}e^{-3t}+c_{3}\cos t+c_{3}\sin t.
            </me></p>
        </example>

        <example>
            <p>Solve
            <me>
            y^{\prime\prime\prime}-3y^{\prime\prime}+3y^{\prime}-y=0.
            </me>
            (Hint: <m>r^{3}-3r^{2}+3r-1=\left(r-1\right)\left(r-1\right)^{2}</m>)</p>
            
            <p>The characteristic polynomial is <m>r^{3}-3r^{2}+3r-1=0</m>
            and by the hint,
            <me>
            \left(r-1\right)^{3}=0
            </me>
            \item So that <m>r=1,1,1</m>
            <me>
            y(t)=c_{1}e^{t}+c_{2}te^{t}+c_{3}t^{2}e^{t}.
            </me></p>
        </example>

        <example>
            <p> Solve 
            <me>
            y^{(4)}+8y^{\prime\prime}-9y=0
            </me>
            (Hint: <m>r^{4}+8r^{2}-9=\left(r^{2}-1\right)\left(r^{2}+9\right)</m>)</p>
            
            <p>By the hint
            <md>
            <mrow>r^{4}+8r^{2}-9 \amp =\left(r^{2}-1\right)\left(r^{2}+9\right)</mrow>
             <mrow>\amp =\left(r-1\right)\left(r+1\right)\left(r-3i\right)\left(r+3i\right).</mrow>
            </md>
            then 
            <me>
            y(t)=c_{1}e^{t}+c_{2}e^{-t}+c_{3}\cos(3t)+c_{4}\sin(3t).
            </me></p>
        </example>

        <example>
            <p>Suppose the roots of the characteristic
            equation are
            <me>
            2,3,3,3,2\pm3i,2\pm3i
            </me>
            then the general solution is
            <md>
            <mrow>y(t) \amp =c_{1}e^{2t}+c_{2}e^{3t}+c_{3}te^{3t}+c_{4}t^{2}e^{3t}</mrow>
             <mrow>\amp +c_{5}e^{2t}\cos(3t)+c_{6}e^{2t}\sin(3t)</mrow>
             <mrow>\amp +c_{5}te^{2t}\cos(3t)+c_{6}te^{2t}\sin(3t).</mrow>
            </md></p>
        </example>
    </subsection>
    </section>



    <section xml:id="ch4-2">
        <title>The Method of Undetermined Coefficients</title>
        <p> We consider 
        <me>
        y^{(n)}+p_{n-1}(t)y^{(n-1)}+\cdots+p_{1}(t)y^{\prime}+p_{0}(t)y=g(t)
        </me>
        where <m>g(t)</m> can be a polynomial, sin, cos, exp or products of these.
        Recall the general solution is of the form: <m>y=y_{h}+y_{p}</m> where
        <m>y_{h}</m> is the general solution of the corresponding homogeneous
        equation and <m>y_{p}</m> is a particular solution to the non-homogeneous
        equation.</p>

        <example> 
            <p>Find the general solution of
            <me>
            y^{\prime\prime\prime}-y^{\prime\prime}-y^{\prime}+y=2e^{-t}+3.
            </me>
            (Hint: <m>r^{3}-r^{2}-r+1=\left(r-1\right)\left(r-1\right)\left(r+1\right)</m>)</p>

            <p>Step 1: We find <m>y_{h}</m>: Solve <m>r^{3}-r^{2}-r+1=0</m>,
            but by the hint
            <me>
            \left(r-1\right)\left(r-1\right)\left(r+1\right)=0
            </me>
            so that <m>y_{h}=c_{1}e^{t}+c_{2}te^{t}+c_{3}e^{-t}</m>.</p>

            <p>Step 2: Find <m>y_{p}</m>: We first guess
            <m>y_{p}=Ae^{-t}+B</m>, but there are repeats with <m>y_{h}</m> hence we get
            a second guess of 
            <md>
            <mrow>y_{p} \amp =Ate^{-t}+B</mrow>
            <mrow>y_{p}^{\prime} \amp =Ae^{-t}-Ate^{-t}</mrow>
            <mrow>y_{p}^{\prime\prime} \amp =-Ae^{-t}-Ae^{-t}+Ate^{-t}=-2Ae^{-t}+Ate^{-t}</mrow>
            <mrow>y_{p}^{\prime\prime\prime} \amp =2Ae^{-t}+Ae^{-t}-Ate^{-t}=3Ae^{-t}-Ate^{-t}</mrow>
            </md>
            Hence 
            <md>
            <mrow>LHS \amp =3Ae^{-t}-Ate^{-t}</mrow>
             <mrow>\amp +2Ae^{-t}-Ate^{-t}</mrow>
             <mrow>\amp -Ae^{-t}+Ate^{-t}</mrow>
             <mrow>\amp +Ate^{-t}+B</mrow>
             <mrow>\amp =4Ae^{-t}+B</mrow>
            </md></p>

            <p>Step 3: Set LHS=RHS so that 
            <me>
            LHS=4Ae^{-t}+B=2e^{-t}+3=RHS
            </me>
            hence 
            <md>
            <mrow>4A=2 \amp ,B=3</mrow>
            <mrow>A=\frac{1}{2}</mrow>
            </md>
            hence 
            <me>
            y_{p}=\frac{1}{2}te^{-t}+3
            </me>
            so that the General Solution is 
            <me>
            y=c_{1}e^{t}+c_{2}te^{t}+c_{3}e^{-t}+\frac{1}{2}te^{-t}+3.
            </me></p>
        </example>
        <example>
            <p>Consider 
            <me>
            y^{\prime\prime\prime}+4y^{\prime}=t+\sin(4t).
            </me>
            Find the general form of <m>y_{p}</m>.</p>

            <p>Step 1: We find <m>y_{h}</m>: Solve 
            <md>
            <mrow>r^{3}+4r \amp =0</mrow>
            <mrow>r\left(r^{2}+4\right) \amp =0</mrow>
            </md>
            so that <m>y_{h}=c_{1}+c_{2}\cos2t+c_{3}\sin2t</m>. </p>

            <p>Step 2: Find <m>y_{p}</m>: 
            We first guess <m>y_{p}=At+B+C\cos(4t)+D\sin(4t)</m>.
            But <m>B</m> is already in <m>y_{c}</m> as <m>c_{1}</m>. So instead make the second guess <m>y_{p}=t\left(At+B\right)+C\cos(4t)+D\sin(4t)</m>
            which is correct. 
            </p>
        </example>

        <example>
            <p>Consider 
            <me>
            y^{(4)}-2y^{\prime\prime}+y=e^{t}+te^{-t}.
            </me>
            Find the general form of <m>y_{p}</m>. (Hint: <m>r^{4}-2r^{2}+1=\left(r^{2}-1\right)^{2}</m>)</p>

            <p>Step 1: We find <m>y_{h}</m>: Solve 
            <md>
            <mrow>r^{4}-2r^{2}+1 \amp =0</mrow>
            <mrow>\left(r^{2}-1\right)^{2} \amp =0</mrow>
            </md>
            so that <m>y_{h}=c_{1}e^{t}+c_{2}te^{t}+c_{3}e^{-t}+c_{4}te^{-t}</m>.</p>
            
            <p>Step 2: Find <m>y_{p}</m>: 
            <ol>
            <li>First guess: <m>y_{p}=Ae^{t}+\left(Bt+C\right)e^{-t}</m>. </li>
            <li> Second Guess: <m>y_{p}=Ate^{t}+\left(Bt^{2}+Ct\right)e^{-t}</m>.</li>
            <li>Third Guess: <m>y_{p}=At^{2}e^{t}+\left(Bt^{3}+Ct^{2}\right)e^{-t}</m>. </li>
            </ol></p>
        </example>

        <example> 
            <p>Suppose 
            <me>
            y^{(5)}=t^{3},
            </me>
            find the general form for <m>y_{p}</m>.</p>
            
            <p>We find <m>y_{h}</m>: The roots to <m>r^{5}=0</m>
            are
            <me>
            r=0,0,0,0,0
            </me>
             so that 
            <me>
            y_{c} =c_{1}+c_{2}t+c_{3}t^{2}+c_{4}t^{3}+c_{4}t^{4}
            </me></p>
         
            <p>Step 2: Find <m>y_{p}</m>:
            <ol>
            <li>First Guess: <m>y_{p}=At^{3}+Bt^{2}+Ct+D</m> </li>
            <li>Final Guess:}} <m>y_{p}=t^{5}\left(At^{3}+Bt^{2}+Ct+D\right)</m> </li>
            </ol></p>
        </example>
    </section>
</chapter>